

$$= \alpha(0) + \beta(0)$$

$$= 0.$$

Linear combination

Let V be a vector space over F .
 And $v_1, v_2, v_3, \dots, v_n \in V$. Any vector v of the form $\alpha_1 v_1 + \alpha_2 v_2 + \dots + \alpha_n v_n$
 $\alpha_1, \alpha_2, \dots, \alpha_n \in F$ is the linear
 combination of a vector v_1, v_2, \dots, v_n .

1. Let $V = \mathbb{R}^2$, $S = \{(1, 2), (2, 1)\}$, $v = (2, 2) \in V$
 and $\alpha, \beta \in F$. Check whether v is the
 linear combination of v_1 and v_2 .

Solution

$$\text{Let } v = \alpha v_1 + \beta v_2$$

$$(2, 2) = \alpha(1, 2) + \beta(2, 1)$$

$$(2, 2) = (\alpha, 2\alpha) + (2\beta, \beta)$$

$$(2, 2) = (\alpha + 2\beta, 2\alpha + \beta) \quad \text{--- (1)}$$

Equating

$$2 = \alpha + 2\beta \quad \text{--- (2)}$$

$$2 = 2\alpha + \beta \quad \text{--- (3)}$$

$$(2) \times 2 \Rightarrow 4 = 2\alpha + 4\beta$$

$$(3) \Rightarrow \underline{2 = 2\alpha + \beta}$$

$$2 = 3\beta$$

$$\beta = \frac{2}{3} \quad \text{--- (3)}$$

Substitute (3) in (2)

$$2 = \alpha + 2\left(\frac{2}{3}\right)$$

$$6 = 3\alpha + 4$$

$$2 = 3\alpha$$

$$\alpha = \frac{2}{3} \quad \text{--- (4)}$$

$$(1) \Rightarrow (2) = \alpha + 2\beta$$

$$2 = \frac{2}{3} + 2\left(\frac{2}{3}\right)$$

$$2 = \frac{2}{3} + \frac{4}{3}$$

$$2 = \frac{6}{3}$$

$$2 = 2$$

Hence 2 is the vector space.

2. Let $V = \mathbb{R}^3$, $S = \{(1, 2, 0), (0, -5, -7)\}$
 $v = (2, -5, 7) \in V$ verify whether v is
linear combination or not.

Solution

$$\text{Let } v = \alpha v_1 + \beta v_2 \dots \gamma v_3$$

$$(2, -5, 7) = \alpha(1, 2, 0) + \beta(0, -5, -7)$$

$$(2, -5, 7) = (\alpha, 2\alpha, 0) + (0, -5\beta, -7\beta)$$

$$(2, -5, 7) = (\alpha + 0, 2\alpha - 5\beta, 0 - 7\beta)$$

$$(2, -5, 7) = (\alpha, 2\alpha - 5\beta, -7\beta)$$

Equations

$$\boxed{2 = \alpha}$$

$$-7 = -7\beta$$

$$\boxed{\beta = -1}$$

$$2(2) - 5(-1) = 4 + 5 = 9$$

$$-5 \neq 9$$

Hence 9 is not a linear combination

3. Determine whether
expressed as a linear
of $u = (1, -3, 2)$ and $v = (2, -1, 1)$ in \mathbb{R}^3 .
solution.

$$\text{Let } v = \alpha u + \beta v$$

$$(1, 7, -4) = \alpha(1, -3, 2) + \beta(2, -1, 1)$$

$$(1, 7, -4) = (\alpha, -3\alpha, 2\alpha) + (2\beta, -\beta, \beta)$$

$$(1, 7, -4) = (\alpha + 2\beta, -3\alpha - \beta, 2\alpha + \beta)$$

Equating

$$\alpha + 2\beta = 1 \quad \text{--- (1)}$$

$$-3\alpha - \beta = 7 \quad \text{--- (2)}$$

$$2\alpha + \beta = -4 \quad \text{--- (3)}$$

$$\alpha = -3$$

$$\beta = 2$$

$$(1) \Rightarrow -3 + 2(2) = 1$$

$$-3 + 4 = 1$$

$$1 = 1$$

Hence v is the linear combination.

* 4. Write a vector $v = (1, -2, 5)$ as the
linear combination of vectors
 $e_1 = (1, 1, 1)$, $e_2 = (1, 2, 3)$, $e_3 = (2, -1, 1)$ in \mathbb{R}^3 .

$$\text{Let } v = \alpha_1 e_1 + \alpha_2 e_2 + \alpha_3 e_3$$

$$(1, -2, 5) = \alpha_1(1, 1, 1) + \alpha_2(1, 2, 3) + \alpha_3(2, -1, 1)$$

$$= (\alpha_1, \alpha_2, \alpha_1) + (\alpha_2, 2\alpha_2, 3\alpha_2) +$$

$$(2\alpha_3, -\alpha_3, \alpha_3)$$

$$(1, -2, 5) = (\alpha_1 + \alpha_2 + 2\alpha_3) + (\alpha_2 + 2\alpha_2 + 3\alpha_3) + (\alpha_1 + 3\alpha_2 + \alpha_3) \quad \text{--- (1)}$$

3 Determine whether R^3 $(1, 7, -4)$ is expressed as a linear combination of $u: (1, -3, 2)$ and $v: (2, -1, 1)$ in R^3 .

Solution

$$\text{Let } v: \alpha_1 u + \beta_1 v$$

$$(1, 7, -4) = \alpha(1, -3, 2) + \beta(2, -1, 1)$$

$$(1, 7, -4) = (\alpha, -3\alpha, 2\alpha) + (2\beta, -\beta, \beta)$$

$$(1, 7, -4) = (\alpha + 2\beta, -3\alpha - \beta, 2\alpha + \beta)$$

Equating

$$\alpha + 2\beta = 1 \quad \text{--- (1)}$$

$$-3\alpha - \beta = 7 \quad \text{--- (2)}$$

$$2\alpha + \beta = -4 \quad \text{--- (3)}$$

$$\alpha = -3$$

$$\beta = 2$$

$$(1) \Rightarrow -3 + 2(2) = 1$$

$$-3 + 4 = 1$$

$$1 = 1$$

Hence 1 is the linear combination.

* 4 Write a vector $v = (1, -2, 5)$ as the linear combination of vectors $e_1 = (1, 1, 1)$, $e_2 = (1, 2, 3)$, $e_3 = (2, -1, 1)$ in R

$$\text{let } v: \alpha_1 e_1 + \alpha_2 e_2 + \alpha_3 e_3$$

$$\begin{aligned} (1, -2, 5) &= \alpha_1(1, 1, 1) + \alpha_2(1, 2, 3) + \alpha_3(2, -1, 1) \\ &= (\alpha_1, \alpha_2, \alpha_1) + (\alpha_2, 2\alpha_2, 3\alpha_2) + (2\alpha_3, -\alpha_3, \alpha_3) \end{aligned}$$

$$\begin{aligned} (1, -2, 5) &= (\alpha_1 + \alpha_2 + 2\alpha_3) + (\alpha_1 + 2\alpha_2 + 3\alpha_3) \\ &\quad + (\alpha_1 + 3\alpha_2 + \alpha_3) \quad \text{--- (1)} \end{aligned}$$

Equating

$$\alpha_1 + \alpha_2 + 2\alpha_3 = 1$$

$$\alpha_1 + 2\alpha_2 + 3\alpha_3 = -2$$

$$\alpha_1 + 3\alpha_2 + \alpha_3 = 5$$

Solving these equations, we get

$$\alpha_1 = -6$$

$$\alpha_2 = 3$$

$$\alpha_3 = 2$$

$$(2) \Rightarrow -6 + 3 + 2(2) = 1$$

$$-6 + 3 + 4 = 1$$

$$-6 + 7 = 1$$

$$1 = 1$$

Hence v is the linear combination.

5. Consider the vectors $(1, 2, 3)$ and $v = (2, 3, 1)$ in \mathbb{R}^3 . For what values of k is the vector $w = (1, k, 4)$ is the linear combination of u and v .

Solution

$$v = \alpha_1 u + \alpha_2 v$$

$$(1, k, 4) = \alpha_1 (1, 2, 3) + \alpha_2 (2, 3, 1)$$

$$(1, k, 4) = (\alpha_1, 2\alpha_1, 3\alpha_1) + (2\alpha_2, 3\alpha_2, \alpha_2)$$

$$(1, k, 4) = (\alpha_1 + 2\alpha_2, 2\alpha_1 + 3\alpha_2, 3\alpha_1 + \alpha_2) \quad \text{--- (1)}$$

$$\alpha_1 + 2\alpha_2 = 1 \quad \text{--- (2)}$$

$$2\alpha_1 + 3\alpha_2 = k \quad \text{--- (3)}$$

$$3\alpha_1 + \alpha_2 = 4 \quad \text{--- (4)}$$

$$\alpha_1 = \frac{7}{5}$$

$$\alpha_2 = -\frac{1}{5}$$

in eqn (3)

$$\Rightarrow 2\left(\frac{7}{5}\right) + 3\left(-\frac{1}{5}\right) = k$$

$$k = \frac{11}{5}$$

6. Consider the vectors $u = (1, 2, -1)$ and $v = (6, 4, 2)$ in \mathbb{R}^3 . Show that $w = (9, 2, 7)$ is the linear combination of u and v .

$$w = \alpha_1 u + \alpha_2 v$$

$$(9, 2, 7) = \alpha_1 (1, 2, -1) + \alpha_2 (6, 4, 2)$$

$$(9, 2, 7) = (\alpha_1, 2\alpha_1, -\alpha_1) + (6\alpha_2, 4\alpha_2, 2\alpha_2)$$

$$(9, 2, 7) = (\alpha_1 + 6\alpha_2, 2\alpha_1 + 4\alpha_2, -\alpha_1 + 2\alpha_2)$$

$$\alpha_1 + 6\alpha_2 = 9 \quad \text{--- (1)}$$

$$2\alpha_1 + 4\alpha_2 = 2 \quad \text{--- (2)}$$

$$-\alpha_1 + 2\alpha_2 = 7 \quad \text{--- (3)}$$

$$\alpha_1 = -3 \quad \alpha_2 = 2$$

$$(1) \Rightarrow -3 + 6(2) = 9$$

$$9 = 9$$

Hence V is the vector space.

7. Check the polynomial $2x^3 - 2x^2 + 12x - 6$ is the linear combination of $3x^3 - 5x^2 - 4x - 9$ and $x^3 - 2x^2 - 5x - 3$ in P_3 .
Solution

$$\text{In } 2x^3 - 2x^2 + 12x - 6 = \alpha_1 (x^3 - 2x^2 - 5x - 3) + \alpha_2 (3x^3 - 5x^2 - 4x - 9)$$

$$2x^3 - 2x^2 + 12x - 6 = (\alpha_1 x^3 - 2\alpha_1 x^2 - 5\alpha_1 x - 3\alpha_1) + (3\alpha_2 x^3 - 5\alpha_2 x^2 - 4\alpha_2 x - 9\alpha_2)$$

$$2x^3 - 2x^2 + 12x - 6 = x^3 (\alpha_1 + 3\alpha_2) + x^2 (-2\alpha_1 - 5\alpha_2) + x (-5\alpha_1 - 4\alpha_2) + (-3\alpha_1 - 9\alpha_2)$$

Equating

--- (1)

$$2 = \alpha_1 + 3\alpha_2 \quad \text{--- (2)}$$

$$-2 = -2\alpha_1 - 5\alpha_2 \quad \text{--- (3)}$$

$$12 = -5\alpha_1 - 4\alpha_2 \quad \text{--- (4)}$$

$$-6 = -3\alpha_1 - 9\alpha_2 \quad \text{--- (5)}$$

$$\alpha_1 = -4$$

$$\alpha_2 = 2$$

$$(2) \Rightarrow -4 + 3(2) = 2$$

$$-4 + 6 = 2$$

$$2 = 2$$

Hence the polynomial is a linear combination.

8. Check the polynomial $3x^3 - 2x^2 + 7x + 8$ is the linear combination of $x^3 - 2x^2 - 5x - 3$ and $3x^3 - 5x^2 - 4x - 9$ in $P_3(x)$

Solution.

$$3x^3 - 2x^2 + 7x + 8 = \alpha_1(x^3 - 2x^2 - 5x - 3) + \alpha_2(3x^3 - 5x^2 - 4x - 9)$$

$$3x^3 - 2x^2 + 7x + 8 = (\alpha_1 x^3 - 2\alpha_1 x^2 - 5\alpha_1 x - 3\alpha_1) + (3\alpha_2 x^3 - 5\alpha_2 x^2 - 4\alpha_2 x - 9\alpha_2)$$

$$3x^3 - 2x^2 + 7x + 8 = x^3(\alpha_1 + 3\alpha_2) + x^2(-2\alpha_1 - 5\alpha_2) + x(-5\alpha_1 - 4\alpha_2) + (3\alpha_1 - 9\alpha_2) \quad \text{--- (1)}$$

Equating

$$\alpha_1 + 3\alpha_2 = 3 \quad \text{--- (2)}$$

$$-2\alpha_1 - 5\alpha_2 = -2 \quad \text{--- (3)}$$

$$-5\alpha_1 - 4\alpha_2 = 7 \quad \text{--- (4)}$$

$$3\alpha_1 - 9\alpha_2 = 8 \quad \text{--- (5)}$$

$$\alpha_1 = -9$$

$$\alpha_2 = 4$$

$$12 = -5(-4) - 4(2)$$

$$12 = +20 - 8$$

$$12 = 12$$

$$-6 = -3(4) - 9(2)$$

$$-6 = -12 - 18$$

$$-6 = -6$$

$$-5(-9) - 4(4) = 7$$

$$45 - 16 = 7$$

$$29 = 7$$

$$3(-9) - 9(4) = 8$$

$$-27 - 36 = 8$$

$$-63 = 8$$

Hence the polynomial is the linear combination.

9. Write the matrix $E = \begin{bmatrix} 3 & 1 \\ 1 & -1 \end{bmatrix}$ as a linear combination of matrices $A: \begin{bmatrix} 1 & 1 \\ 1 & 0 \end{bmatrix}$, $B: \begin{bmatrix} 0 & 0 \\ 1 & 1 \end{bmatrix}$, $C: \begin{bmatrix} 0 & 2 \\ 0 & -1 \end{bmatrix}$.

Solution

$$\text{Let } E = \alpha_1 A + \alpha_2 B + \alpha_3 C \quad \text{--- (1)}$$

$$\begin{bmatrix} 3 & 1 \\ 1 & -1 \end{bmatrix} = \alpha_1 \begin{bmatrix} 1 & 1 \\ 1 & 0 \end{bmatrix} + \alpha_2 \begin{bmatrix} 0 & 0 \\ 1 & 1 \end{bmatrix} + \alpha_3 \begin{bmatrix} 0 & 2 \\ 0 & -1 \end{bmatrix}$$

$$= \begin{bmatrix} \alpha_1 & \alpha_1 \\ \alpha_1 & 0 \end{bmatrix} + \begin{bmatrix} 0 & 0 \\ \alpha_2 & \alpha_2 \end{bmatrix} + \begin{bmatrix} 0 & 2\alpha_3 \\ 0 & -\alpha_3 \end{bmatrix}$$

$$\begin{bmatrix} 3 & 1 \\ 1 & -1 \end{bmatrix} = \begin{bmatrix} \alpha_1 & \alpha_1 + 2\alpha_3 \\ \alpha_1 + \alpha_2 & \alpha_2 - \alpha_3 \end{bmatrix}$$

Equating

$$\alpha_1 = 3 \quad \text{--- (1)}$$

$$\alpha_1 + 2\alpha_3 = 1 \quad \text{--- (2)}$$

$$\alpha_1 + \alpha_2 = 1 \quad \text{--- (3)}$$

$$\alpha_2 - \alpha_3 = -1 \quad \text{--- (4)}$$

$$(3) \Rightarrow \alpha_2 + 3 = 1$$

$$\alpha_2 = 1 - 3$$

$$\alpha_2 = -2$$

$$(4) \Rightarrow \alpha_2 - \alpha_3 = -1$$

$$-2 - \alpha_3 = -1$$

$$-\alpha_3 = -1 + 2$$

$$\alpha_3 = -1$$

$$(2) \Rightarrow 3 + 2(-1) = 1$$

$$3 - 2 = 1$$

$$1 = 1$$

$$(I) E = 3A - 2B - C$$

Linear Span

Definition.

Let V be a vector space over a field F and S be a non empty subset of V . Then the set of all linear combination of the finite subset S is called the linear span of S . And it is denoted by $L(S)$.

$$(ii) L(S) = \{ \alpha_1 v_1 + \alpha_2 v_2 + \dots + \alpha_n v_n \mid \alpha_i \in F, v_i \in S \}$$

Note.

$$* L(S) \subseteq V$$

$$* \text{ If } S = \emptyset, \text{ then } L(S) = 0.$$

1. Let $S = \{(1, 2), (2, 1)\}$, $V = \mathbb{R}^2$. Prove that V is the linear span of S .

Solution

$$\text{We know that } L(S) \subseteq V \quad \text{--- (1)}$$

Let us consider $(x, y) \in V$.

$$(x, y) \in V$$

$$(x, y) = \alpha_1(1, 2) + \alpha_2(2, 1) \quad \text{--- (2)}$$

$$= (\alpha_1, 2\alpha_1) + (2\alpha_2, \alpha_2)$$

$$(x, y) = (\alpha_1 + 2\alpha_2, 2\alpha_1 + \alpha_2)$$

Equating on both sides

$$\alpha_1 + 2\alpha_2 = x \quad \text{--- (3)}$$

$$2\alpha_1 + \alpha_2 = y \quad \text{--- (4)}$$

$$(2) \Rightarrow 2\alpha_1 + 4\alpha_2 = 2x$$

$$(4) \Rightarrow 2\alpha_1 + \alpha_2 = -y$$

$$3\alpha_2 = 2x - y$$

$$\alpha_2 = \frac{2x - y}{3}$$

$$(3) \Rightarrow \alpha_1 + 2\left[\frac{2x - y}{3}\right] = x$$

$$3\alpha_1 + 4x - 2y = 3x$$

$$3\alpha_1 = 3x - 4x + 2y$$

$$3\alpha_1 = -x + 2y$$

$$\alpha_1 = \frac{2y - x}{3}$$

Sub α_1, α_2 in (2)

$$(x, y) = \left(\frac{2y - x}{3}\right)(1, 2) + \left(\frac{2x - y}{3}\right)(2, 1)$$

Hence x, y is the linear combination of S .

$$\therefore (x, y) \in L(S)$$

$$(x, y) \in V \Rightarrow (x, y) \in L(S)$$

$$\therefore V \subseteq L(S) \text{ --- (5)}$$

From (1), (2)

$$L(S) = V.$$

the S generates V .

2. Prove that $V_2(R)$, $(3, 7) \in$ linear span $\{(1, 2), (0, 1)\}$

Let $S: \{(1, 2), (0, 1)\}$

$$v_1 = (1, 2)$$

$$v_2 = (0, 1)$$

$$\begin{aligned}\therefore V &= \alpha_1 V_1 + \alpha_2 V_2 \\ (x, y) &= \alpha_1 (1, 2) + \alpha_2 (0, 1) \quad \text{--- (1)} \\ &= (\alpha_1, 2\alpha_1) + (0, \alpha_2) \\ (x, y) &= (\alpha_1, 2\alpha_1 + \alpha_2)\end{aligned}$$

Equating

$$\alpha_1 = x$$

$$2\alpha_1 + \alpha_2 = y$$

$$\alpha_2 = y - 2\alpha_1$$

$$(1) \Rightarrow (x, y) = x(1, 2) + (y - 2x)(0, 1)$$

check $(3, 7) \in L(S)$

Here $x = 3, y = 7$

$$\begin{aligned}(3, 7) &= 3(1, 2) + (7 - 2(3))(0, 1) \\ &= (3, 6) + (7 - 6)(0, 1) \\ &= (3, 6) + (0, 1) \\ &= (3, 6) + (0, 1)\end{aligned}$$

$$(3, 7) = (3, 7)$$

Which is true:

$$\therefore (3, 7) \in L(S)$$

3. Determine whether the set of vectors $x_1 = (1, 1, 2), x_2 = (1, 0, 1), x_3 = (2, 1, 3)$ span \mathbb{R}^3 .

$$\text{Let } S = \{(1, 1, 2), (1, 0, 1), (2, 1, 3)\}$$

$$\text{WKT. } L(S) \subseteq \mathbb{R}^3 \quad \text{--- (1)}$$

$$\text{Let } V \in \mathbb{R}^3, V = (a, b, c)$$

$$V = \alpha_1 V_1 + \alpha_2 V_2 + \alpha_3 V_3$$

$$\begin{aligned}(a, b, c) &= \alpha_1 (1, 1, 2) + \alpha_2 (1, 0, 1) + \alpha_3 (2, 1, 3) \\ &= (\alpha_1, \alpha_1, 2\alpha_1) + (\alpha_2, 0, \alpha_2) + (2\alpha_3, \alpha_3, 3\alpha_3)\end{aligned}$$

$$\begin{aligned}(a, b, c) &= (\alpha_1 + \alpha_2 + 2\alpha_3, \alpha_1 + \alpha_3, 2\alpha_1 + \alpha_2 + 3\alpha_3)\end{aligned}$$

$$\therefore V = \alpha_1 V_1 + \alpha_2 V_2$$

$$(x, y) = \alpha_1 (1, 2) + \alpha_2 (0, 1) \quad \text{--- (1)}$$

$$= (\alpha_1, 2\alpha_1) + (0, \alpha_2)$$

$$(x, y) = (\alpha_1, 2\alpha_1 + \alpha_2)$$

Equating

$$\alpha_1 = x$$

$$2\alpha_1 + \alpha_2 = y$$

$$\alpha_2 = y - 2\alpha_1$$

$$(1) \Rightarrow (x, y) = x(1, 2) + (y - 2x)(0, 1)$$

Check $(3, 7) \in L(S)$

Here $x = 3, y = 7$

$$(3, 7) = 3(1, 2) + (7 - 2(3))(0, 1)$$

$$= (3, 6) + (7 - 6)(0, 1)$$

$$= (3, 6) + (0, 1)$$

$$= (3, 6) + (0, 1)$$

$$(3, 7) = (3, 7)$$

Which is true:

$$\therefore (3, 7) \in L(S)$$

3. Determine whether the set of vectors

$$x_1 = (1, 1, 2), x_2 = (1, 0, 1), x_3 = (2, 1, 3)$$

Span \mathbb{R}^3 .

$$\text{Let } S = \{(1, 1, 2), (1, 0, 1), (2, 1, 3)\}$$

$$\text{WKT, } L(S) \subseteq \mathbb{R}^3 \quad \text{--- (1)}$$

$$\text{Let } V \in \mathbb{R}^3, V = (a, b, c)$$

$$V = \alpha_1 V_1 + \alpha_2 V_2 + \alpha_3 V_3$$

$$(a, b, c) = \alpha_1 (1, 1, 2) + \alpha_2 (1, 0, 1) + \alpha_3 (2, 1, 3)$$

$$= (\alpha_1, \alpha_1, 2\alpha_1) + (\alpha_2, 0, \alpha_2) + (2\alpha_3, \alpha_3, 3\alpha_3)$$

$$(a, b, c) = (\alpha_1 + \alpha_2 + 2\alpha_3, \alpha_1 + 0\alpha_2 + \alpha_3, 2\alpha_1 + \alpha_2 + 3\alpha_3)$$

Equating

$$\alpha_1 + \alpha_2 + 2\alpha_3 = a \quad (2)$$

$$\alpha_1 + 0\alpha_2 + \alpha_3 = b \quad (3)$$

$$2\alpha_1 + \alpha_2 + 3\alpha_3 = c \quad (4)$$

Solve (1), (2), (3)

$$\begin{bmatrix} 1 & 1 & 2 \\ 1 & 0 & 1 \\ 2 & 1 & 3 \end{bmatrix} \begin{bmatrix} \alpha_1 \\ \alpha_2 \\ \alpha_3 \end{bmatrix} = \begin{bmatrix} a \\ b \\ c \end{bmatrix}$$

$$[A, B] \sim \left[\begin{array}{ccc|c} 1 & 1 & 2 & a \\ 1 & 0 & 1 & b \\ 2 & 1 & 3 & c \end{array} \right] \begin{array}{l} R_2 \rightarrow R_2 - R_1 \\ R_3 \rightarrow R_3 - 2R_1 \end{array}$$

$$[A, B] \sim \left[\begin{array}{ccc|c} 1 & 1 & 2 & a \\ 0 & -1 & -1 & b-a \\ 0 & -1 & -1 & c-2a \end{array} \right] \begin{array}{l} R_2 \rightarrow R_2 - R_1 \\ R_3 \rightarrow R_3 - 2R_2 \end{array}$$

$$\alpha_1 + \alpha_2 + 2\alpha_3 = a$$

$$0\alpha_1 - \alpha_2 - \alpha_3 = b - a$$

$$[A, B] \sim \left[\begin{array}{ccc|c} 1 & 1 & 2 & a \\ 0 & -1 & -1 & b-a \\ 0 & 0 & 0 & c-a-b \end{array} \right] R_3 \rightarrow R_3 - R_2$$

$$0\alpha_1 + 0\alpha_2 + 0\alpha_3 = c - a - b - b$$

$$0 = c - a - b$$

Which is not possible.

Given vector does not span R^3

Gen

4. Prove that the vectors $(1, 1, 0)$, $(1, 0, 1)$, $(0, 1, 1)$ generate R^3 .

Solution.

Generate: A subset S of a subs vector space generate (or) span V , if $L(S) = V$.

$$\text{Let } S = \{(1, 1, 0), (1, 0, 1), (0, 1, 1)\}$$

$$\text{W.K.T } L(S) \subseteq \mathbb{R}^3 \text{ — (1)}$$

$$\text{Let } v \in \mathbb{R}^3, v = (a, b, c)$$

$$v = \alpha_1 v_1 + \alpha_2 v_2 + \alpha_3 v_3$$

$$(a, b, c) = \alpha_1 (1, 1, 0) + \alpha_2 (1, 0, 1) + \alpha_3 (0, 1, 1)$$

$$= (\alpha_1, \alpha_1, 0\alpha_1) + (\alpha_2, 0\alpha_2, \alpha_2) + (0\alpha_3, \alpha_3, \alpha_3)$$

$$(a, b, c) = (\alpha_1 + \alpha_2 + 0\alpha_3, \alpha_1 + 0\alpha_2 + \alpha_3, 0\alpha_1 + \alpha_2 + \alpha_3)$$

$$\alpha_1 + \alpha_2 + 0\alpha_3 = a \text{ — (2)}$$

$$\alpha_1 + 0\alpha_2 + \alpha_3 = b \text{ — (3)}$$

$$0\alpha_1 + \alpha_2 + \alpha_3 = c \text{ — (4)}$$

$$\left[\begin{array}{ccc|c} 1 & 1 & 0 & \alpha_1 \\ 1 & 0 & 1 & \alpha_2 \\ 0 & 1 & 1 & \alpha_3 \end{array} \right] = \left[\begin{array}{c} a \\ b \\ c \end{array} \right]$$

$$[A, B] \sim \left[\begin{array}{ccc|c} 1 & 1 & 0 & a \\ 1 & 0 & 1 & b \\ 0 & 1 & 1 & c \end{array} \right]$$

$$\sim \left[\begin{array}{ccc|c} 1 & 1 & 0 & a \\ 0 & -1 & 1 & b-a \\ 0 & 1 & 1 & c \end{array} \right] R_2 \rightarrow R_2 - R_1$$

$$\sim \left[\begin{array}{ccc|c} 1 & 1 & 0 & a \\ 0 & -1 & 1 & b-a \\ 0 & 0 & 2 & c+b-a \end{array} \right] R_3 \rightarrow R_3 + R_2$$

$$2\alpha_3 = c + b - a \text{ — (5)}$$

$$-\alpha_2 + \alpha_3 = b - a \text{ — (6)}$$

$$\alpha_1 + \alpha_2 = a \text{ — (7)}$$

$$(5) \Rightarrow \alpha_3 = \frac{1}{2}(c + b - a)$$

$$(6) \Rightarrow -\alpha_2 + \alpha_3 = b - a$$

$$\alpha_2 = -b + a + \alpha_3$$

$$\alpha_2 = -b + a + \frac{1}{2}(c + b - a)$$

$$= \frac{1}{2}(-2b + 2a + c + b - a)$$

$$\alpha_2 = \frac{1}{2}(-b + a + c)$$

$$(7) \Rightarrow \alpha_1 + \frac{1}{2}(-b+a+c) = a$$

$$\alpha_1 = a - \frac{1}{2}(-b+a+c)$$

$$\alpha_1 = \frac{1}{2}(2a+b-a-c)$$

$$\alpha_1 = \frac{1}{2}(a+b-c)$$

substitute the values of $\alpha_1, \alpha_2, \alpha_3$ in (9)

$$(9) \Rightarrow v = \frac{1}{2}(a+b-c)(1,1,0) + \frac{1}{2}(a+c-b)(1,0,1) + \frac{1}{2}(c+b-a)(0,1,1)$$

$$v \in L(S)$$

$$\therefore R^3 \subseteq L(S) \quad \text{--- (8)}$$

From (1) & (8)

We get, $L(S) = R^3$.

$\therefore S$ generates R^3 .

Prove that the polynomials (x^2+3x-2) , $(2x^2+5x-3)$ and $(-x^2-4x+4)$ generates $P_2(R)$.

$$\text{Let } S = \{p(x), q(x), r(x)\}$$

$$L(S) \subseteq P_2(R) \quad \text{--- (1)}$$

$$t(x) \in P_2(R)$$

$$\text{then } t(x) = ax^2+bx+c$$

$$\text{Let } t(x) = \alpha_1 p(x) + \alpha_2 q(x) + \alpha_3 r(x)$$

$$ax^2+bx+c = \alpha_1(x^2+3x-2) + \alpha_2(2x^2+5x-3) + \alpha_3(-x^2-4x+4) \quad \text{--- (2)}$$

$$= (\alpha_1 x^2 + 3\alpha_1 x - 2\alpha_1) + (2\alpha_2 x^2 + 5\alpha_2 x - 3\alpha_2) + (\alpha_3 x^2 - 4\alpha_3 x + 4\alpha_3)$$

$$ax^2+bx+c = x^2(\alpha_1 + 2\alpha_2 - \alpha_3) + (3\alpha_1 + 5\alpha_2 - 4\alpha_3)x + (-2\alpha_1 - 3\alpha_2 + 4\alpha_3)$$

$$x_1 + 2x_2 - x_3 = a \quad \text{--- (2)}$$

$$3x_1 + 5x_2 - 4x_3 = b \quad \text{--- (3)}$$

$$-2x_1 - 3x_2 + 4x_3 = c \quad \text{--- (4)}$$

$$\begin{bmatrix} 1 & 2 & -1 \\ 3 & 5 & -4 \\ -2 & -3 & 4 \end{bmatrix} \begin{bmatrix} x_1 \\ x_2 \\ x_3 \end{bmatrix} = \begin{bmatrix} a \\ b \\ c \end{bmatrix}$$

$$[A, B] \sim \left[\begin{array}{ccc|c} 1 & 2 & -1 & a \\ 3 & 5 & -4 & b \\ -2 & -3 & 4 & c \end{array} \right]$$

$$\sim \left[\begin{array}{ccc|c} 1 & 2 & -1 & a \\ 0 & -1 & -1 & b-3a \\ 0 & 1 & 2 & c+2a \end{array} \right] \begin{array}{l} R_2 \rightarrow R_2 - 3R_1 \\ R_3 \rightarrow R_3 + 2R_1 \end{array}$$

$$\sim \left[\begin{array}{ccc|c} 1 & 2 & -1 & a \\ 0 & -1 & -1 & b-3a \\ 0 & 0 & 1 & c+b-a \end{array} \right] R_3 \rightarrow R_3 + R_2$$

$$x_3 = c + b - a \quad \text{--- (5)}$$

$$-x_2 - x_3 = b - 3a \quad \text{--- (6)}$$

$$x_1 + 2x_2 - x_3 = a \quad \text{--- (7)}$$

$$(5) \Rightarrow x_3 = c + b - a$$

$$(6) \Rightarrow x_2 = x_3 + b - 3a$$

$$x_2 = -x_3 - b + 3a$$

$$x_2 = -(c + b - a) - b + 3a$$

$$= -c - b + a - b + 3a$$

$$x_2 = 4a - 2b - c$$

$$(7) \Rightarrow x_1 + 2x_2 - x_3 = a$$

$$x_1 = a - 2x_2 + x_3$$

$$= a - 2(4a - 2b - c) + (c + b - a)$$

$$= a - 8a + 4b + 2c + c + b - a$$

$$x_1 = -8a + 5b + 3c$$

substitute eqns 1, 2, 3 in 7

$$(ax^2+bx+c) = (-8a+5b+3c)(x^2+3x-2) \\ (4a-2b-c)(2x^2+5x-3) \\ (c+b-a)(-x^2-4x+4)$$

$$P_2(R) \subseteq L(S) \text{ --- (8)}$$

From (1) & (8)

$$L(S) = P_2(R)$$

$\therefore S$ generate $P_2(R)$